src3.0/Vellvm/Dominators/dom_tree.v
@@ -54,6 +54,11 @@ match chain with
 | _ => dt
 end.
 
+Definition create_dtree_from_chains pe (chains:list (A * list A)) : DTree :=
+fold_left 
+  (fun acc elt => create_dtree_from_chain acc (snd elt))
+  chains (DT_node pe DT_nil).
+
 Fixpoint in_children_roots child dts : bool :=
 match dts with
 | DT_nil => false
@@ -173,7 +178,32 @@ forall ch tl p0 ch0,
   is_dtrees_edge (dtrees_insert dts ch tl) p0 ch0 = true <->
   is_dtrees_edge dts p0 ch0 = true \/ is_chain_edge (ch::tl) p0 ch0.
 
-Lemma is_dtrees_egde_cons_elim: forall dt1 dts2 p ch
+Lemma is_dtree_edge_node_elim: forall a1 dts2 p ch
+  (Hin: is_dtree_edge (DT_node a1 dts2) p ch = true),
+  (a1 = p /\ in_children_roots ch dts2 = true) \/ 
+  is_dtrees_edge dts2 p ch = true.
+Proof.
+  simpl.
+  intros.
+  destruct_if; auto.
+  destruct_if; auto.
+Qed.
+
+Lemma is_dtree_edge_node_intro: forall a1 dts2 p ch
+  (Hintro: (a1 = p /\ in_children_roots ch dts2 = true) \/ 
+           is_dtrees_edge dts2 p ch = true),
+  is_dtree_edge (DT_node a1 dts2) p ch = true.
+Proof.
+  simpl.
+  intros.
+  destruct Hintro as [[EQ Hin] | Hedge]; subst.
+    destruct_if.
+    destruct_if; congruence.
+
+    destruct_if. destruct_if.
+Qed.
+
+Lemma is_dtrees_edge_cons_elim: forall dt1 dts2 p ch
   (Hin: is_dtrees_edge (DT_cons dt1 dts2) p ch = true),
   is_dtree_edge dt1 p ch = true \/ is_dtrees_edge dts2 p ch = true.
 Proof.
@@ -182,7 +212,7 @@ Proof.
   binvt Hin as J1 J2; auto.
 Qed.
 
-Lemma is_dtrees_egde_cons_intro: forall dt1 dts2 p ch
+Lemma is_dtrees_edge_cons_intro: forall dt1 dts2 p ch
   (Hin: is_dtree_edge dt1 p ch = true \/ is_dtrees_edge dts2 p ch = true),
   is_dtrees_edge (DT_cons dt1 dts2) p ch = true.
 Proof.
@@ -210,12 +240,12 @@ Local Opaque is_dtrees_edge.
       destruct (list2tree_spec hd tl') as [x Heq].
       rewrite Heq in H0.
       destruct (Hdec hd ch0); subst; auto.
-        apply is_dtrees_egde_cons_elim in H0.
+        apply is_dtrees_edge_cons_elim in H0.
         destruct H0 as [H0 | H0].
           right. apply IHtl'. rewrite Heq. auto.
 
           rewrite DT_nil_has_no_dtree_edges in H0. congruence.
-       apply is_dtrees_egde_cons_elim in H0.
+       apply is_dtrees_edge_cons_elim in H0.
        destruct H0 as [H0 | H0].
          right. apply IHtl'. auto.
          rewrite DT_nil_has_no_dtree_edges in H0. congruence.
@@ -236,10 +266,10 @@ Proof.
 
       destruct (Hdec p0 ch); subst.
         destruct (Hdec hd ch0); subst; auto.
-          apply is_dtrees_egde_cons_intro.
+          apply is_dtrees_edge_cons_intro.
           left. rewrite <- Heq. apply IHtl'; auto.          
 
-        apply is_dtrees_egde_cons_intro.
+        apply is_dtrees_edge_cons_intro.
         left. rewrite <- Heq. apply IHtl'; auto.          
 Transparent is_dtrees_edge.
 Qed.
@@ -324,7 +354,7 @@ Proof.
       SSCase "tl<>nil".
         split; intro J.
         SSSCase "1".
-          apply is_dtrees_egde_cons_elim in J.
+          apply is_dtrees_edge_cons_elim in J.
           destruct J as [J | J].
           SSSSCase "1.1".
             apply H in J. 
@@ -333,7 +363,7 @@ Proof.
           SSSSCase "1.2".
             left. rewrite J. auto with datatypes v62.
         SSSCase "2".
-          apply is_dtrees_egde_cons_intro.
+          apply is_dtrees_edge_cons_intro.
           destruct J as [J | [[J1 J2] | J]]; subst.
           SSSSCase "2.1".
             binvt J as J1 J2; auto.
@@ -345,18 +375,18 @@ Proof.
     SCase "l0 <> ch".
         split; intro J.
         SSSCase "1".
-          apply is_dtrees_egde_cons_elim in J.
+          apply is_dtrees_edge_cons_elim in J.
           destruct J as [J | J].
           SSSSCase "1.1".
             left.
-            apply is_dtrees_egde_cons_intro; auto.
+            apply is_dtrees_edge_cons_intro; auto.
           SSSSCase "1.2".
             apply H0 in J.
             destruct J as [J | J].
-              left. apply is_dtrees_egde_cons_intro; auto.
+              left. apply is_dtrees_edge_cons_intro; auto.
               right. auto.
         SSSCase "2".
-          apply is_dtrees_egde_cons_intro.
+          apply is_dtrees_edge_cons_intro.
           destruct J as [J | J].    
           SSSSCase "2.1".
             binvt J as J1 J2; auto.
@@ -425,7 +455,7 @@ Lemma fold_left_create_dtree_from_chain__is_dtree_edge__is_chain_edge:
   (is_dtree_edge
     (fold_left
       (fun (acc : DTree) (elt : A * list A) =>
-       let '(_, chain) := elt in create_dtree_from_chain acc chain)
+       create_dtree_from_chain acc (snd elt))
      chains dt) p0 ch0 = true ->
   (is_dtree_edge dt p0 ch0 = true \/
    exists l0, exists chain0,
@@ -437,7 +467,7 @@ Lemma fold_left_create_dtree_from_chain__is_dtree_edge__is_chain_edge:
    is_dtree_edge
     (fold_left
       (fun (acc : DTree) (elt : A * list A) =>
-       let '(_, chain) := elt in create_dtree_from_chain acc chain)
+       create_dtree_from_chain acc (snd elt))
      chains dt) p0 ch0 = true).
 Proof.
   induction chains as [|[p l1] chains]; simpl; intros.
@@ -465,6 +495,27 @@ Proof.
 
           right. exists l2. exists chain2. split; auto. split; auto.
             apply create_dtree_from_chain__chain_connects_dtree; auto.
+Qed.
+
+Lemma create_dtree_from_chains__is_dtree_edge__is_chain_edge: forall pe chains
+  p0 ch0,
+  (is_dtree_edge (create_dtree_from_chains pe chains) p0 ch0 = true ->
+  (exists l0, exists chain0,
+     List.In (l0, chain0) chains /\ is_chain_edge chain0 p0 ch0)) /\
+  ((exists l0, exists chain0,
+     List.In (l0, chain0) chains /\ 
+     chain_connects_dtree (DT_node pe DT_nil) chain0 /\
+     is_chain_edge chain0 p0 ch0) ->
+   is_dtree_edge (create_dtree_from_chains pe chains) p0 ch0 = true).
+Proof.
+  unfold create_dtree_from_chains.
+  intros.
+  destruct (fold_left_create_dtree_from_chain__is_dtree_edge__is_chain_edge
+    p0 ch0 chains (DT_node pe DT_nil)) as [J1 J2].
+  split; intros J; auto.
+    apply J1 in J.
+    destruct J as [J | J]; auto.
+      simpl in J. destruct (Hdec p0 pe); tinv J.
 Qed.
 
 Lemma is_chain_edge_tail: forall p0 ch0 ls2 ls1 
@@ -576,15 +627,136 @@ with disjoint_children_dtrees : DTrees -> Prop :=
                disjoint_children_dtrees (DT_cons dt dts)
 .
 
-Definition dtree_is_sound (dt:DTree) (idom: A -> A -> Prop): Prop :=
-  forall p ch (Hedge: is_dtree_edge dt p ch = true),
-    exists chain, is_chain_edge chain p ch /\ 
-    Sorted idom chain /\ NoDup chain.
+Definition dtree_insert__disjoint_children_prop (dt:DTree) :=
+forall p ch tl (Hdisj: disjoint_children_dtree dt),
+  disjoint_children_dtree (dtree_insert dt p ch tl).
 
-Definition dtrees_is_sound (dts:DTrees) (idom: A -> A -> Prop) : Prop :=
-  forall p ch (Hedge: is_dtrees_edge dts p ch = true),
-    exists chain, is_chain_edge chain p ch /\ 
-    Sorted idom chain /\ NoDup chain.
+Definition dtrees_insert__disjoint_children_prop (dts:DTrees) :=
+forall ch tl (Hdisj: disjoint_children_dtrees dts),
+  disjoint_children_dtrees (dtrees_insert dts ch tl).
+
+Lemma list2tree__disjoint_children_dtree: forall (tl : list A) (ch : A),
+  disjoint_children_dtree (list2tree ch tl).
+Proof.
+  induction tl; simpl; intros.
+    repeat constructor. 
+    repeat constructor; auto.
+Qed. 
+
+Lemma list2tree__disjoint_dtrees_roots: forall ch tl,
+  disjoint_dtrees_roots (DT_cons (list2tree ch tl) DT_nil).
+Proof.
+  destruct tl; simpl; auto.
+Qed.
+
+Lemma dtrees_insert__notin_get_dtrees_roots: forall a ch tl (Hneq: a <> ch)
+  dts (Hnotin: ~ In a (get_dtrees_roots dts)),
+  ~ In a (get_dtrees_roots (dtrees_insert dts ch tl)).
+Proof.
+  induction dts as [|[] dts]; simpl; intros.
+    destruct tl; simpl; intro J; destruct J; subst; auto.
+
+    destruct_if; simpl.
+      destruct tl; simpl; auto.
+      destruct_if.
+    
+      intro J.
+      apply set_add_elim in J.
+      destruct J as [J | J]; subst.
+        apply Hnotin. apply set_add_intro2; auto.
+
+        apply Hnotin. apply set_add_intro1.
+        destruct (In_dec Hdec a (get_dtrees_roots dts)) as [H | H]; auto.
+        apply IHdts in H. tauto.
+Qed.
+
+Lemma dtrees_insert__disjoint_dtrees_roots: forall ch tl dts
+  (Hdisj: disjoint_dtrees_roots dts),
+  disjoint_dtrees_roots (dtrees_insert dts ch tl).
+Proof.
+  induction dts as [|[] dts]; simpl; intros; auto.
+    destruct_if.
+      destruct tl; simpl; auto.
+      destruct_if.
+    
+      simpl.
+      destruct Hdisj.
+      split; auto using dtrees_insert__notin_get_dtrees_roots.
+Qed.
+
+Lemma dtree_insert__disjoint_children_mutrec :
+  (forall dt, dtree_insert__disjoint_children_prop dt) *
+  (forall dts, dtrees_insert__disjoint_children_prop dts).
+Proof.
+  apply dtree_mutrec;
+    unfold dtree_insert__disjoint_children_prop, 
+           dtrees_insert__disjoint_children_prop;
+    intros; simpl.
+  Case "DT_node".
+    destruct_if. 
+    inv Hdisj.
+    constructor; auto.
+  Case "DT_nil".
+    constructor; auto using list2tree__disjoint_children_dtree,
+                            list2tree__disjoint_dtrees_roots.
+  Case "DT_cons".
+    destruct d. 
+    destruct_if. 
+      destruct tl; auto.
+      inv Hdisj.
+      constructor; auto.
+        simpl.
+        destruct_if. 
+
+      inv Hdisj.
+      constructor; auto.
+        simpl in Hdisj0.
+        destruct Hdisj0 as [J1 J2].
+        simpl.
+        split.
+          apply dtrees_insert__notin_get_dtrees_roots; auto.
+          apply dtrees_insert__disjoint_dtrees_roots; auto.
+Qed.
+
+Lemma dtree_insert__disjoint_children: forall (dt:DTree) p ch tl 
+  (Hdisj: disjoint_children_dtree dt),
+  disjoint_children_dtree (dtree_insert dt p ch tl).
+Proof.
+  intros.
+  destruct dtree_insert__disjoint_children_mutrec as [J1 J2].
+  apply J1; auto.
+Qed.
+
+Lemma create_dtree_from_chain__disjoint_children: forall (dt:DTree) chain
+  (Hdisj: disjoint_children_dtree dt),
+  disjoint_children_dtree (create_dtree_from_chain dt chain).
+Proof.
+  intros.
+  do 2 (destruct chain; auto). 
+  simpl.
+  apply dtree_insert__disjoint_children; auto.
+Qed.
+
+Lemma fold_left_create_dtree_from_chain__disjoint_children:
+  forall chains dt (Hdisj: disjoint_children_dtree dt),
+  disjoint_children_dtree 
+    (fold_left
+      (fun (acc : DTree) (elt : A * list A) =>
+       create_dtree_from_chain acc (snd elt))
+     chains dt).
+Proof.
+  induction chains as [|[p l1] chains]; simpl; intros; auto.
+    apply IHchains. apply create_dtree_from_chain__disjoint_children; auto.
+Qed.
+
+Lemma create_dtree_from_chains__disjoint_children_dtree: forall pe chains,
+  disjoint_children_dtree (create_dtree_from_chains pe chains).
+Proof.
+  unfold create_dtree_from_chains.
+  intros.
+  apply fold_left_create_dtree_from_chain__disjoint_children.
+    do 2 constructor.
+Qed.
 
 Fixpoint in_children (dt: DTree) dts : Prop :=
 match dts with
@@ -663,6 +835,51 @@ Lemma get_dtree_root_in_dtree_dom: forall dt,
 Proof.
   destruct dt; simpl.
   apply set_add_intro2; auto.
+Qed.
+
+Lemma in_dtree_dom_intro1: forall a dts,
+  In a (dtree_dom (DT_node a dts)).
+Proof.
+  intros.
+  assert (J:=get_dtree_root_in_dtree_dom (DT_node a dts)).
+  auto.
+Qed.
+
+Lemma in_dtree_dom_intro2: forall a x dts (Hin: In x (dtrees_dom dts)),
+  In x (dtree_dom (DT_node a dts)).
+Proof.
+  induction dts; simpl; intros; auto.
+    apply set_add_intro1.
+    apply set_union_intro.
+    apply set_union_elim in Hin.
+    destruct Hin as [Hin | Hin]; auto.
+Qed.
+
+Lemma in_dtrees_dom_intro1: forall x dt dts (Hin: In x (dtree_dom dt)),
+  In x (dtrees_dom (DT_cons dt dts)).
+Proof.
+  intros. simpl. apply set_union_intro; auto.
+Qed.
+
+Lemma in_dtrees_dom_intro2: forall x dt dts (Hin: In x (dtrees_dom dts)),
+  In x (dtrees_dom (DT_cons dt dts)).
+Proof.
+  intros. simpl. apply set_union_intro; auto.
+Qed.
+
+Lemma in_dtree_dom_elim: forall a x dts (Hin: In x (dtree_dom (DT_node a dts))),
+  x = a \/ In x (dtrees_dom dts).
+Proof.
+  simpl. intros.
+  apply set_add_elim in Hin; auto.
+Qed.
+
+Lemma in_dtrees_dom_elim: forall x dt dts 
+  (Hin: In x (dtrees_dom (DT_cons dt dts))),
+  In x (dtree_dom dt) \/ In x (dtrees_dom dts).
+Proof.
+  simpl. intros. 
+  apply set_union_elim in Hin; auto.
 Qed.
 
 Lemma dtree_child_walk__dtree_walk: forall l1 l2 dt dts 
@@ -798,13 +1015,39 @@ Proof.
         rewrite IHdts; auto with datatypes v62.
 Qed.
 
+
+Lemma notin_get_dtrees_roots__neq: forall a dt dts
+  (Hnotin: ~ In a (get_dtrees_roots dts))
+  (Hin: in_children dt dts),
+  a <> get_dtree_root dt.
+Proof.
+  induction dts; simpl; intros.
+    tauto.
+
+    destruct Hin as [Hin | Hin]; subst.
+      intro EQ. subst.
+      apply Hnotin. apply set_add_intro2; auto.
+
+      intro EQ. subst. 
+      apply IHdts; auto.
+        intro J. apply Hnotin. apply set_add_intro1; auto.
+Qed.
+
+Definition dtree_is_sound (dt:DTree) (idom: A -> A -> Prop): Prop :=
+  forall p ch (Hedge: is_dtree_edge dt p ch = true),
+    exists chain, is_chain_edge chain p ch /\ Sorted idom chain.
+
+Definition dtrees_is_sound (dts:DTrees) (idom: A -> A -> Prop) : Prop :=
+  forall p ch (Hedge: is_dtrees_edge dts p ch = true),
+    exists chain, is_chain_edge chain p ch /\ Sorted idom chain.
+
 Lemma dtree_edge_sorted: forall R dt p ch
   (Hp : dtree_is_sound dt R) (Hedge: is_dtree_edge dt p ch = true),
   R p ch.
 Proof.
   intros.
   apply Hp in Hedge.
-  destruct Hedge as [chain [J1 [J2 J3]]].
+  destruct Hedge as [chain [J1 J2]].
   eapply chain_edge_sorted; eauto.
 Qed.
 
@@ -833,8 +1076,8 @@ Proof.
   unfold dtree_is_sound, dtrees_is_sound in *.
   intros.
   split; intros.
-    apply Hp. apply is_dtrees_egde_cons_intro; auto.
-    apply Hp. apply is_dtrees_egde_cons_intro; auto.
+    apply Hp. apply is_dtrees_edge_cons_intro; auto.
+    apply Hp. apply is_dtrees_edge_cons_intro; auto.
 Qed.
 
 Lemma dtrees_is_sound__dtree_is_sound: forall dt idom dts
@@ -851,23 +1094,6 @@ Proof.
       apply IHdts; auto.
         intros p0 ch0 Hedge0.
         apply H. rewrite Hedge0. auto with datatypes v62.
-Qed.
-
-Lemma notin_get_dtrees_roots__neq: forall a dt dts
-  (Hnotin: ~ In a (get_dtrees_roots dts))
-  (Hin: in_children dt dts),
-  a <> get_dtree_root dt.
-Proof.
-  induction dts; simpl; intros.
-    tauto.
-
-    destruct Hin as [Hin | Hin]; subst.
-      intro EQ. subst.
-      apply Hnotin. apply set_add_intro2; auto.
-
-      intro EQ. subst. 
-      apply IHdts; auto.
-        intro J. apply Hnotin. apply set_add_intro1; auto.
 Qed.
 
 Lemma dtree_walk__clos_refl_trans_idom: forall idom dt l1 (Hwk: dtree_walk dt l1)
@@ -935,6 +1161,10 @@ Implicit Arguments forall_parent_children [A].
 Implicit Arguments disjoint_dtrees [A].
 Implicit Arguments disjoint_dtrees_roots [A].
 Implicit Arguments dtree_walk [A].
+Implicit Arguments get_dtree_root_in_dtree_dom [A].
+Implicit Arguments list2tree [A].
+Implicit Arguments create_dtree_from_chains [A].
+Implicit Arguments create_dtree_from_chains__is_dtree_edge__is_chain_edge [A].
 
 Require Import Maps.
 
@@ -962,6 +1192,7 @@ with reachable_dtrees : @DTrees T.elt -> Prop :=
                  reachable_dtrees (DT_cons dt dts)
 .
 
+
 Lemma reachable_dtree__reachable_root: forall d 
   (Hreach: reachable_dtree d),
   TCfg.reachable succs entry (get_dtree_root d).
@@ -983,20 +1214,174 @@ Qed.
 Import AtomSet.
 Import ListSet.
 
-Definition in_dom_tree_is_reachable_prop (dt:DTree) :=
+Definition reachable_dtree_intro_prop (dt:DTree) :=
+  forall (Hintro: forall x (Hp: In x (dtree_dom Hdec dt)), 
+                           TCfg.reachable succs entry x), 
+  reachable_dtree dt.
+
+Definition reachable_dtrees_intro_prop (dts:DTrees) :=
+  forall (Hintro: forall x (Hp: In x (dtrees_dom Hdec dts)),
+                           TCfg.reachable succs entry x), 
+  reachable_dtrees dts.
+      
+Lemma reachable_dtree_intro_mutrec :
+  (forall dt, reachable_dtree_intro_prop dt) *
+  (forall dts, reachable_dtrees_intro_prop dts).
+Proof.
+  apply dtree_mutrec;
+    unfold reachable_dtree_intro_prop, reachable_dtrees_intro_prop;
+    simpl; intros. 
+  Case "NODE".
+    constructor.
+      apply Hintro; auto using in_dtree_dom_intro1.
+
+      apply H. intros.
+      apply Hintro; auto using in_dtree_dom_intro2.
+  Case "NIL".
+    constructor.
+  Case "CONS".
+    constructor.
+      apply H; intros.
+      apply Hintro.
+
+      unfold dtrees_dom.
+      apply set_union_intro; auto.
+
+      apply H0; intros.
+      apply Hintro.
+      unfold dtrees_dom.
+      apply set_union_intro; auto.
+Qed.
+
+Lemma reachable_dtree_intro: forall (dt:DTree)
+  (Hintro: forall x (Hp: In x (dtree_dom Hdec dt)), 
+                           TCfg.reachable succs entry x), 
+  reachable_dtree dt.
+Proof.
+  intros. 
+  destruct reachable_dtree_intro_mutrec as [J1 J2]. 
+  apply J1; auto.
+Qed.
+
+Lemma reachable_dtrees_intro: forall (dts:DTrees)
+  (Hintro: forall x (Hp: In x (dtrees_dom Hdec dts)),
+                           TCfg.reachable succs entry x), 
+  reachable_dtrees dts.
+Proof.
+  intros. 
+  destruct reachable_dtree_intro_mutrec as [J1 J2]. 
+  apply J2; auto.
+Qed.
+
+Definition dtree_insert__reachable_dtree_prop (dt:DTree) :=
+forall p ch tl (Hrd: reachable_dtree dt)
+  (Hrd': forall x (Hin: In x (p::ch::tl)), TCfg.reachable succs entry x),
+  reachable_dtree (dtree_insert Hdec dt p ch tl).
+
+Definition dtrees_insert__reachable_dtrees_prop (dts:DTrees) :=
+forall ch tl (Hrd: reachable_dtrees dts)
+  (Hrd': forall x (Hin: In x (ch::tl)), TCfg.reachable succs entry x),
+  reachable_dtrees (dtrees_insert Hdec dts ch tl).
+
+Lemma list2tree__reachable_dtree: forall tl ch
+  (Hrd: forall x (Hin: In x (ch::tl)), TCfg.reachable succs entry x),
+  reachable_dtree (list2tree ch tl).
+Proof.
+  induction tl; simpl; intros.
+    repeat constructor; auto.
+    repeat constructor; auto.
+Qed. 
+
+Lemma dtree_insert__reachable_dtree_mutrec :
+  (forall dt, dtree_insert__reachable_dtree_prop dt) *
+  (forall dts, dtrees_insert__reachable_dtrees_prop dts).
+Proof.
+  apply dtree_mutrec;
+    unfold dtree_insert__reachable_dtree_prop, 
+           dtrees_insert__reachable_dtrees_prop;
+    intros; simpl.
+  Case "DT_node".
+    destruct_if. 
+    inv Hrd.
+    constructor; auto.
+      apply H; auto.
+        intros x Hinx. apply Hrd'. auto with datatypes v62.
+  Case "DT_nil".
+    constructor; auto using list2tree__reachable_dtree.
+  Case "DT_cons".
+    destruct d. 
+    destruct_if. 
+      destruct tl; auto.
+      inv Hrd.
+      constructor; auto.
+
+      inv Hrd.
+      constructor; auto.
+Qed.
+
+Lemma dtree_insert__reachable_dtree: forall (dt:DTree) 
+  p ch tl (Hrd: reachable_dtree dt)
+  (Hrd': forall x (Hin: In x (p::ch::tl)), TCfg.reachable succs entry x),
+  reachable_dtree (dtree_insert Hdec dt p ch tl).
+Proof.
+  intros.
+  destruct dtree_insert__reachable_dtree_mutrec as [J1 J2].
+  apply J1; auto.
+Qed.
+
+Definition reachable_chain chain :=
+forall x (Hin: In x chain), TCfg.reachable succs entry x.
+
+Lemma create_dtree_from_chain__reachable_dtree: forall (dt:DTree) chain
+  (Hrd: reachable_dtree dt) (Hrd': reachable_chain chain),
+  reachable_dtree (create_dtree_from_chain Hdec dt chain).
+Proof.
+  intros.
+  do 2 (destruct chain; auto). 
+  simpl.
+  apply dtree_insert__reachable_dtree; auto.
+Qed.
+
+Lemma fold_left_create_dtree_from_chain__reachable_dtree:
+  forall (chains:list (T.elt * list T.elt)) dt (Hrd: reachable_dtree dt)
+  (Hrd': Forall (fun elt => reachable_chain (snd elt)) chains),
+  reachable_dtree 
+    (fold_left
+      (fun (acc : DTree) elt => create_dtree_from_chain Hdec acc (snd elt))
+     chains dt).
+Proof.
+  induction chains as [|[p l1] chains]; simpl; intros; auto.
+    inv Hrd'.
+    apply IHchains; auto.
+    apply create_dtree_from_chain__reachable_dtree; auto.
+Qed.
+
+Lemma create_dtree_from_chains__reachable_dtree: forall chains
+  (Hincfg: TCfg.XTree.in_cfg succs entry)
+  (Hrd: Forall (fun elt => reachable_chain (snd elt)) chains),
+  reachable_dtree (create_dtree_from_chains Hdec entry chains).
+Proof.
+  unfold create_dtree_from_chains.
+  intros.
+  apply fold_left_create_dtree_from_chain__reachable_dtree; auto.
+    repeat constructor.
+      apply TCfg.reachable_entry; auto.
+Qed.
+
+Definition reachable_dtree_elim_prop (dt:DTree) :=
   forall (Hrd: reachable_dtree dt) x (Hp: In x (dtree_dom Hdec dt)), 
     TCfg.reachable succs entry x.
 
-Definition in_dom_trees_is_reachable_prop (dts:DTrees) :=
+Definition reachable_dtrees_elim_prop (dts:DTrees) :=
   forall (Hrd: reachable_dtrees dts) x (Hp: In x (dtrees_dom Hdec dts)), 
     TCfg.reachable succs entry x.
 
-Lemma in_dom_tree_is_reachable_mutrec :
-  (forall dt, in_dom_tree_is_reachable_prop dt) *
-  (forall dts, in_dom_trees_is_reachable_prop dts).
+Lemma reachable_dtree_elim_mutrec :
+  (forall dt, reachable_dtree_elim_prop dt) *
+  (forall dts, reachable_dtrees_elim_prop dts).
 Proof.
   apply dtree_mutrec;
-    unfold in_dom_tree_is_reachable_prop, in_dom_trees_is_reachable_prop;
+    unfold reachable_dtree_elim_prop, reachable_dtrees_elim_prop;
     simpl; intros; inv Hrd.
   Case "NODE".
     unfold dtree_dom in Hp.
@@ -1010,14 +1395,32 @@ Proof.
     destruct Hp as [Hp | Hp]; auto.
 Qed.
 
+Lemma reachable_dtree_elim: forall (dt:DTree)
+  (Hrd: reachable_dtree dt) x (Hp: In x (dtree_dom Hdec dt)), 
+  TCfg.reachable succs entry x.
+Proof.
+  intros. 
+  destruct reachable_dtree_elim_mutrec as [J1 J2].
+  eapply J1; eauto.
+Qed.
+
+Lemma  reachable_dtrees_elim: forall (dts:DTrees)
+  (Hrd: reachable_dtrees dts) x (Hp: In x (dtrees_dom Hdec dts)), 
+  TCfg.reachable succs entry x.
+Proof.
+  intros. 
+  destruct reachable_dtree_elim_mutrec as [J1 J2].
+  eapply J2; eauto.
+Qed.
+
 Lemma inter_reachable_dtree_is_reachable: forall dt dts
   (Hwfdt : reachable_dtree dt) (Hwfdts : reachable_dtrees dts) (x : T.elt) 
   (Hinx : In x (set_inter Hdec (dtree_dom Hdec dt) (dtrees_dom Hdec dts))),
   TCfg.reachable succs entry x.
 Proof.
   intros. 
-  destruct in_dom_tree_is_reachable_mutrec as [J1 J2].
-  unfold in_dom_tree_is_reachable_prop, in_dom_trees_is_reachable_prop in *.
+  destruct reachable_dtree_elim_mutrec as [J1 J2].
+  unfold reachable_dtree_elim_prop, reachable_dtrees_elim_prop in *.
   apply set_inter_elim in Hinx.
   destruct Hinx; eauto.
 Qed.
@@ -1175,3 +1578,593 @@ Qed.
 End create_dtree__wf_dtree.
 
 End DTreeProps.
+
+Module PDProps := DTreeProps(PTree).
+Module ADProps := DTreeProps(ATree).
+
+Module DTreeConv.
+(* This module may be able to define with parameters source and target TREEs.
+   Say DTreeConv (S:TREE) (T:TREE).
+   Then inside DTreeConv, we can 
+ 
+   Module SProps := DTreeProps(S).
+   Module TProps := DTreeProps(T).
+   ...
+
+   But, when do
+   Module A := DTreeConv(PTree)(ATree).
+   The inductive type A.SProps.wf_dtree and ADProps.wf_dtree are not
+   convertable directively. None inductive types are fine. 
+  
+   In general,
+
+   Module A := DTreeProps(ATree).
+   Module A' := DTreeProps(ATree).
+   Coq does not think A.wf_dtree and A'.wf_dtree are the same, although we 
+   can prove that they are equivalent manually.
+
+   We should solve the problem to generalize DTreeConv.
+*) 
+
+Section DTreeConv.
+
+Variable s2t:PTree.t ATree.elt.
+Hypothesis Tdec: forall x y:ATree.elt, {x = y} + {x <> y}.
+Hypothesis Sdec: forall x y:PTree.elt, {x = y} + {x <> y}.
+
+Fixpoint sdtree_tdtree (sdt: @DTree PTree.elt) : option (@DTree ATree.elt) :=
+match sdt with
+| DT_node s sdts => 
+    match PTree.get s s2t, sdtrees_tdtrees sdts with
+    | Some t, Some tdts => Some (DT_node t tdts)
+    | _, _ => None
+    end
+end
+with sdtrees_tdtrees (sdts: @DTrees PTree.elt) : option (@DTrees ATree.elt) :=
+match sdts with
+| DT_nil => Some DT_nil
+| DT_cons sdt sdts => 
+    match sdtree_tdtree sdt, sdtrees_tdtrees sdts with
+    | Some tdt, Some tdts => Some (DT_cons tdt tdts)
+    | _, _ => None
+    end
+end.
+
+Definition sdtree_tdtree_is_total_prop (sdt:DTree) :=
+  forall (s2t_is_total: 
+           forall s (Hin: In s (dtree_dom Sdec sdt)), PTree.get s s2t <> None),
+  sdtree_tdtree sdt <> None.
+
+Definition sdtrees_tdtrees_is_total_prop (sdts:DTrees) :=
+  forall (s2t_is_total: 
+           forall s (Hin: In s (dtrees_dom Sdec sdts)), PTree.get s s2t <> None),
+  sdtrees_tdtrees sdts <> None.
+
+Lemma sdtree_tdtree_is_total_mutrec :
+  (forall sdt, sdtree_tdtree_is_total_prop sdt) *
+  (forall sdts, sdtrees_tdtrees_is_total_prop sdts).
+Proof.
+  apply dtree_mutrec;
+    unfold sdtree_tdtree_is_total_prop, sdtrees_tdtrees_is_total_prop;
+    simpl; intros.
+  Case "1".
+    case_eq (PTree.get a s2t).
+      intros e Heq.
+      case_eq (sdtrees_tdtrees d); try congruence.
+        intros Heq'.
+        contradict Heq'.
+        apply H.
+        intros s Hins.
+        apply s2t_is_total.
+        apply in_dtree_dom_intro2; auto.
+      intro Heq.
+      contradict Heq.
+      apply s2t_is_total.
+      apply in_dtree_dom_intro1; auto.
+  Case "2".
+    congruence.
+  Case "3".
+    case_eq (sdtree_tdtree d).
+      intros e Heq.
+      case_eq (sdtrees_tdtrees d0); try congruence.
+        intros Heq'.
+        contradict Heq'.
+        apply H0.
+        intros s Hins.
+        apply s2t_is_total.
+        apply in_dtrees_dom_intro2; auto.
+      intro Heq.
+      contradict Heq.
+      apply H.
+      intros s Hins.
+      apply s2t_is_total.
+      apply in_dtrees_dom_intro1; auto.
+Qed.
+
+Lemma sdtree_tdtree_is_total: forall (sdt:DTree) 
+  (s2t_is_total: forall s (Hin: In s (dtree_dom Sdec sdt)), PTree.get s s2t <> None),
+  sdtree_tdtree sdt <> None.
+Proof.
+  intros.
+  destruct sdtree_tdtree_is_total_mutrec as [J1 J2].
+  apply J1; auto.
+Qed.
+
+Definition in_tdtree_dom__in_sdtree_dom_prop (sdt:DTree) :=
+  forall tdt (Hconv: sdtree_tdtree sdt = Some tdt) 
+    s t (Hget: PTree.get s s2t = Some t),
+    (In t (dtree_dom Tdec tdt) <-> In s (dtree_dom Sdec sdt)).
+
+Definition in_tdtrees_dom__in_sdtrees_dom_prop (sdts:DTrees) :=
+  forall tdts (Hconv: sdtrees_tdtrees sdts = Some tdts)
+    s t (Hget: PTree.get s s2t = Some t),
+    (In t (dtrees_dom Tdec tdts) <-> In s (dtrees_dom Sdec sdts)).
+
+Hypothesis s2t_injective: forall s1 s2 t (Hget1: PTree.get s1 s2t = Some t)
+  (Hgets: PTree.get s2 s2t = Some t), s1 = s2.
+
+Lemma in_tdtree_dom__in_sdtree_dom_mutrec :
+  (forall sdt, in_tdtree_dom__in_sdtree_dom_prop sdt) *
+  (forall sdts, in_tdtrees_dom__in_sdtrees_dom_prop sdts).
+Proof.
+  apply dtree_mutrec;
+    unfold in_tdtree_dom__in_sdtree_dom_prop, 
+           in_tdtrees_dom__in_sdtrees_dom_prop;
+    simpl; intros.
+  Case "node".
+    inv_mbind.
+    split; intro Hin.
+      apply in_dtree_dom_elim in Hin.
+      destruct Hin as [EQ | Hin]; subst.
+        assert (s = a) as EQ.
+          eapply s2t_injective; eauto.
+        subst.
+        apply in_dtree_dom_intro1.
+
+        apply in_dtree_dom_intro2.
+          eapply H; eauto.
+
+      apply in_dtree_dom_elim in Hin.
+        destruct Hin as [EQ | Hin]; subst.
+        rewrite Hget in HeqR. inv HeqR.
+        apply in_dtree_dom_intro1. 
+
+        apply in_dtree_dom_intro2.
+          eapply H; eauto.
+  Case "nil".
+    inv Hconv. split; intro Hin; inv Hin.
+  Case "cons".
+    inv_mbind.
+    split; intro Hin;
+      apply in_dtrees_dom_elim in Hin;
+      destruct Hin as [Hin | Hin]; try solve [
+        apply in_dtrees_dom_intro1; eapply H; eauto |
+        apply in_dtrees_dom_intro2; eapply H0; eauto
+      ].
+Qed.
+
+Lemma in_tdtree_dom__in_sdtree_dom: forall (sdt:DTree) tdt 
+  (Hconv: sdtree_tdtree sdt = Some tdt) s t
+  (Hget: PTree.get s s2t = Some t),
+  (In t (dtree_dom Tdec tdt) <-> In s (dtree_dom Sdec sdt)).
+Proof.
+  intros.
+  destruct in_tdtree_dom__in_sdtree_dom_mutrec as [J1 J2].
+  eapply J1; eauto.
+Qed.
+
+Lemma in_tdtrees_dom__in_sdtrees_dom: forall (sdts:DTrees) tdts
+  (Hconv: sdtrees_tdtrees sdts = Some tdts) s t
+  (Hget: PTree.get s s2t = Some t),
+  (In t (dtrees_dom Tdec tdts) <-> In s (dtrees_dom Sdec sdts)).
+Proof.
+  intros.
+  destruct in_tdtree_dom__in_sdtree_dom_mutrec as [J1 J2].
+  eapply J2; eauto.
+Qed.
+
+Definition in_tdtree_dom__ex_in_sdtree_dom_prop (sdt:DTree) :=
+  forall tdt (Hconv: sdtree_tdtree sdt = Some tdt) 
+    t (Hin: In t (dtree_dom Tdec tdt)),
+    exists s, PTree.get s s2t = Some t /\ In s (dtree_dom Sdec sdt).
+
+Definition in_tdtrees_dom__ex_in_sdtrees_dom_prop (sdts:DTrees) :=
+  forall tdts (Hconv: sdtrees_tdtrees sdts = Some tdts) 
+    t (Hin: In t (dtrees_dom Tdec tdts)),
+    exists s, PTree.get s s2t = Some t /\ In s (dtrees_dom Sdec sdts).
+
+Lemma in_tdtree_dom__ex_in_sdtree_dom_mutrec :
+  (forall sdt, in_tdtree_dom__ex_in_sdtree_dom_prop sdt) *
+  (forall sdts, in_tdtrees_dom__ex_in_sdtrees_dom_prop sdts).
+Proof.
+  apply dtree_mutrec;
+    unfold in_tdtree_dom__ex_in_sdtree_dom_prop, 
+           in_tdtrees_dom__ex_in_sdtrees_dom_prop;
+    simpl; intros.
+  Case "node".
+    inv_mbind.
+    apply in_dtree_dom_elim in Hin.
+    destruct Hin as [EQ | Hin]; subst.
+      exists a. split; auto.
+      apply in_dtree_dom_intro1.
+
+      apply H in Hin; auto.
+      destruct Hin as [s [J1 J2]].
+      exists s. split; auto.
+      apply in_dtree_dom_intro2; auto.
+  Case "nil".
+    inv Hconv. inv Hin.
+  Case "cons".
+    inv_mbind.
+    apply in_dtrees_dom_elim in Hin.
+    destruct Hin as [Hin | Hin].
+      apply H in Hin; auto.
+      destruct Hin as [s [J1 J2]].
+      exists s. split; auto.
+      apply in_dtrees_dom_intro1; auto.
+
+      apply H0 in Hin; auto.
+      destruct Hin as [s [J1 J2]].
+      exists s. split; auto.
+      apply in_dtrees_dom_intro2; auto.
+Qed.
+
+Lemma in_tdtree_dom__ex_in_sdtree_dom: forall (sdt:DTree) tdt 
+  (Hconv: sdtree_tdtree sdt = Some tdt) t (Hin: In t (dtree_dom Tdec tdt)),
+  exists s, PTree.get s s2t = Some t /\ In s (dtree_dom Sdec sdt).
+Proof.
+  intros.
+  destruct in_tdtree_dom__ex_in_sdtree_dom_mutrec as [J1 J2].
+  eapply J1; eauto.
+Qed.
+
+Lemma in_tdtrees_dom__ex_in_sdtrees_dom: forall (sdts:DTrees) tdts
+  (Hconv: sdtrees_tdtrees sdts = Some tdts) t 
+  (Hin: In t (dtrees_dom Tdec tdts)),
+  exists s, PTree.get s s2t = Some t /\ In s (dtrees_dom Sdec sdts).
+Proof.
+  intros.
+  destruct in_tdtree_dom__ex_in_sdtree_dom_mutrec as [J1 J2].
+  eapply J2; eauto.
+Qed.
+
+Lemma disjpint_sdtrees__disjpint_tdtrees: forall (sdts:DTrees) tdts 
+  (Hwf: disjoint_dtrees Sdec sdts) (Hconv: sdtrees_tdtrees sdts = Some tdts),
+  disjoint_dtrees Tdec tdts.
+Proof.
+  induction sdts; simpl; intros.
+    inv Hconv; auto.
+
+    inv_mbind. simpl.
+    destruct Hwf as [J1 J2].
+    split; auto.
+      unfold AtomSet.set_disjoint.
+      destruct J1 as [J1 J3].
+      split; intros x Hinx.
+        apply ListSet.set_inter_elim in Hinx.
+        destruct Hinx as [Hin1 Hin2].
+        eapply in_tdtree_dom__ex_in_sdtree_dom in Hin1; eauto.
+        destruct Hin1 as [s1 [Hget1 Hin1]].
+        eapply in_tdtrees_dom__ex_in_sdtrees_dom in Hin2; eauto.
+        destruct Hin2 as [s2 [Hget2 Hin2]].
+        assert (s1 = s2) as EQ.
+          eapply s2t_injective; eauto.
+        subst.
+        assert (In s2 (ListSet.empty_set PTree.elt)) as Hfalse.
+          apply J1. apply ListSet.set_inter_intro; auto.
+        inv Hfalse.
+
+        inv Hinx.
+Qed.
+
+Lemma in_tchildren__in_schildren: forall (sdts:DTrees) tdt tdts 
+  (Hconv : sdtrees_tdtrees sdts = Some tdts) (Hin : in_children tdt tdts),
+  exists sdt, in_children sdt sdts /\ sdtree_tdtree sdt = Some tdt.
+Proof.
+  induction sdts; simpl; intros.
+    inv Hconv. inv Hin.
+
+    inv_mbind.
+    simpl in Hin.
+    inv Hin.
+      exists d. split; auto.
+
+      eapply IHsdts in H; eauto.
+      destruct H as [sdt [H1 H2]].
+      exists sdt. split; auto.
+Qed.
+
+Lemma sdtree_tdtree__s2t_get_dtree_root: forall sdt tdt
+  (Hconv: sdtree_tdtree sdt = Some tdt),
+  PTree.get (get_dtree_root sdt) s2t = Some (get_dtree_root tdt).
+Proof.
+  destruct sdt; simpl; intros.
+  inv_mbind.
+  simpl. auto.
+Qed.
+
+Lemma in_tchildren_roots__in_schildren_roots: forall t (sdts:DTrees) tdts 
+  (Hconv : sdtrees_tdtrees sdts = Some tdts) 
+  (Hin : in_children_roots Tdec t tdts = true),
+  exists s, in_children_roots Sdec s sdts = true /\ PTree.get s s2t = Some t.
+Proof.
+  induction sdts as [|[] sdts]; simpl; intros.
+    inv Hconv. inv Hin.
+
+    inv_mbind.
+    simpl in Hin.
+    destruct_if.
+      exists e. 
+      destruct_if.
+
+      rewrite H0.
+      eapply IHsdts in H0; eauto.
+      destruct H0 as [s [H1 H2]].
+      exists s. 
+      destruct_if.
+Qed.
+
+Definition is_tdtree_edge__ex_is_sdtree_prop (sdt:DTree) :=
+  forall tdt 
+  (Hconv: sdtree_tdtree sdt = Some tdt) tp tch
+  (Hedge: is_dtree_edge Tdec tdt tp tch = true),
+  exists sp, exists sch, 
+    PTree.get sp s2t = Some tp /\ PTree.get sch s2t = Some tch /\
+    is_dtree_edge Sdec sdt sp sch = true.
+
+Definition is_tdtrees_edge__ex_is_sdtrees_prop (sdts:DTrees) :=
+  forall tdts 
+  (Hconv: sdtrees_tdtrees sdts = Some tdts) tp tch
+  (Hedge: is_dtrees_edge Tdec tdts tp tch = true),
+  exists sp, exists sch, 
+    PTree.get sp s2t = Some tp /\ PTree.get sch s2t = Some tch /\
+    is_dtrees_edge Sdec sdts sp sch = true.
+
+Lemma is_tdtree_edge__ex_is_sdtree_mutrec :
+  (forall sdt, is_tdtree_edge__ex_is_sdtree_prop sdt) *
+  (forall sdts, is_tdtrees_edge__ex_is_sdtrees_prop sdts).
+Proof.
+  apply dtree_mutrec;
+    unfold is_tdtree_edge__ex_is_sdtree_prop, 
+           is_tdtrees_edge__ex_is_sdtrees_prop;
+    intros.
+  Case "node".
+    simpl in Hconv. inv_mbind.
+    apply is_dtree_edge_node_elim in Hedge.
+    destruct Hedge as [[EQ Hin] | Hedge]; subst.
+      eapply in_tchildren_roots__in_schildren_roots in Hin; eauto.
+      destruct Hin as [sch [Hin Hget]].
+      exists a. exists sch.
+      split; auto.
+      split; auto.
+        apply is_dtree_edge_node_intro; auto.
+
+      apply H in Hedge; auto.
+      destruct Hedge as [sp [sch [? [? ?]]]].
+      exists sp. exists sch. 
+      split; auto.
+      split; auto.
+        apply is_dtree_edge_node_intro; auto.
+  Case "nil".
+    inv Hconv. inv Hedge.
+  Case "cons".
+    simpl in Hconv. inv_mbind.
+    apply is_dtrees_edge_cons_elim in Hedge.
+    destruct Hedge as [Hedge | Hedge].
+      apply H in Hedge; auto.
+      destruct Hedge as [sp [sch [? [? ?]]]].
+      exists sp. exists sch. 
+      split; auto.
+      split; auto.
+        apply is_dtrees_edge_cons_intro; auto.
+ 
+      apply H0 in Hedge; auto.
+      destruct Hedge as [sp [sch [? [? ?]]]].
+      exists sp. exists sch. 
+      split; auto.
+      split; auto.
+        apply is_dtrees_edge_cons_intro; auto.     
+Qed.
+
+Lemma is_tdtree_edge__ex_is_sdtree_edge: forall (sdt:DTree) tdt 
+  (Hconv: sdtree_tdtree sdt = Some tdt) tp tch
+  (Hedge: is_dtree_edge Tdec tdt tp tch = true),
+  exists sp, exists sch, 
+    PTree.get sp s2t = Some tp /\ PTree.get sch s2t = Some tch /\
+    is_dtree_edge Sdec sdt sp sch = true.
+Proof.
+  intros.
+  destruct is_tdtree_edge__ex_is_sdtree_mutrec as [J1 J2].
+  eapply J1; eauto.
+Qed.
+
+Lemma in_schildren_roots__in_tchildren_roots: forall t (sdts:DTrees) tdts 
+  (Hconv : sdtrees_tdtrees sdts = Some tdts) s
+  (Hin : in_children_roots Sdec s sdts = true) (Hget: PTree.get s s2t = Some t),
+  in_children_roots Tdec t tdts = true.
+Proof.
+  induction sdts as [|[] sdts]; simpl; intros.
+    inv Hconv. inv Hin.
+
+    inv_mbind.
+    destruct_if.
+      rewrite Hget in HeqR1. inv HeqR1.
+      simpl.
+      destruct_if.
+
+      rewrite H0.
+      simpl.
+      destruct_if.
+      eapply IHsdts in H0; eauto.     
+Qed.
+
+Definition is_sdtree_edge__is_tdtree_edge_prop (sdt:DTree) :=
+  forall tdt (Hconv: sdtree_tdtree sdt = Some tdt) tp tch sp sch
+  (Hedge: is_dtree_edge Sdec sdt sp sch = true)
+  (Hgetp: PTree.get sp s2t = Some tp) (Hgetch: PTree.get sch s2t = Some tch),
+  is_dtree_edge Tdec tdt tp tch = true.
+
+Definition is_sdtrees_edge__is_tdtrees_edge_prop (sdts:DTrees) :=
+  forall tdts (Hconv: sdtrees_tdtrees sdts = Some tdts) tp tch sp sch
+  (Hedge: is_dtrees_edge Sdec sdts sp sch = true)
+  (Hgetp: PTree.get sp s2t = Some tp) (Hgetch: PTree.get sch s2t = Some tch),
+  is_dtrees_edge Tdec tdts tp tch = true.
+
+Lemma is_sdtree_edge__is_tdtree_edge_mutrec :
+  (forall sdt, is_sdtree_edge__is_tdtree_edge_prop sdt) *
+  (forall sdts, is_sdtrees_edge__is_tdtrees_edge_prop sdts).
+Proof.
+  apply dtree_mutrec;
+    unfold is_sdtree_edge__is_tdtree_edge_prop, 
+           is_sdtrees_edge__is_tdtrees_edge_prop;
+    intros.
+  Case "node".
+    simpl in Hconv. inv_mbind.
+    apply is_dtree_edge_node_elim in Hedge.
+    destruct Hedge as [[EQ Hin] | Hedge]; subst.
+      rewrite Hgetp in HeqR. inv HeqR.
+      eapply in_schildren_roots__in_tchildren_roots in Hin; eauto 1.
+      apply is_dtree_edge_node_intro; auto.
+
+      eapply H in Hedge; eauto 1.
+      apply is_dtree_edge_node_intro; auto.
+  Case "nil".
+    inv Hconv. inv Hedge.
+  Case "cons".
+    simpl in Hconv. inv_mbind.
+    apply is_dtrees_edge_cons_elim in Hedge.
+    destruct Hedge as [Hedge | Hedge].
+      eapply H in Hedge; eauto 1.
+      apply is_dtrees_edge_cons_intro; auto.
+
+      apply is_dtrees_edge_cons_intro.
+      right.
+      eapply H0 in Hedge; eauto 1.
+Qed.
+
+Lemma is_sdtree_edge__is_tdtree_edge: forall (sdt:DTree) tdt 
+  (Hconv: sdtree_tdtree sdt = Some tdt) tp tch sp sch
+  (Hedge: is_dtree_edge Sdec sdt sp sch = true)
+  (Hgetp: PTree.get sp s2t = Some tp) (Hgetch: PTree.get sch s2t = Some tch),
+  is_dtree_edge Tdec tdt tp tch = true.
+Proof.
+  intros.
+  destruct is_sdtree_edge__is_tdtree_edge_mutrec as [J1 J2].
+  eapply J1; eauto.
+Qed.
+
+Variable ssuccs: PTree.t (list PTree.elt).
+Variable sentry: PTree.elt.
+Variable tsuccs: ATree.t (list ATree.elt).
+Variable tentry: ATree.elt.
+
+Hypothesis reachable_s2t: forall s t (Hconv: Some t = PTree.get s s2t)
+  (Hrd : PCfg.reachable ssuccs sentry s),
+  ACfg.reachable tsuccs tentry t.
+
+Hypothesis idom_s2t: forall s1 t1 s2 t2 
+  (Hconv1: PTree.get s1 s2t = Some t1) (Hconv2: PTree.get s2 s2t = Some t2)
+  (Hidom: PDProps.idom ssuccs sentry s1 s2),
+  ADProps.idom tsuccs tentry t1 t2.
+
+Definition wf_sdtree__wf_tdtree_prop (sdt:DTree) :=
+  forall (Hwf: PDProps.wf_dtree ssuccs sentry Sdec sdt) tdt 
+    (Hconv: sdtree_tdtree sdt = Some tdt),
+  ADProps.wf_dtree tsuccs tentry Tdec tdt.
+
+Definition wf_sdtrees__wf_tdtrees_prop (sdts:DTrees) :=
+  forall (Hwf: PDProps.wf_dtrees ssuccs sentry Sdec sdts) tdts 
+    (Hconv: sdtrees_tdtrees sdts = Some tdts),
+  ADProps.wf_dtrees tsuccs tentry Tdec tdts.
+
+Lemma wf_sdtree__wf_tdtree_mutrec :
+  (forall sdt, wf_sdtree__wf_tdtree_prop sdt) *
+  (forall sdts, wf_sdtrees__wf_tdtrees_prop sdts).
+Proof.
+  apply dtree_mutrec;
+    unfold wf_sdtree__wf_tdtree_prop, wf_sdtrees__wf_tdtrees_prop;
+    simpl; intros.
+  Case "node".
+    inv_mbind.
+    inv Hwf.
+    constructor; auto.
+    SCase "1".
+      eapply reachable_s2t; eauto.
+    SCase "2".
+      intro Hin. apply Hnotin.
+      eapply in_tdtrees_dom__in_sdtrees_dom; eauto.
+    SCase "3".
+      eapply disjpint_sdtrees__disjpint_tdtrees; eauto.
+    SCase "4".
+      apply in_children__forall_parent_children.
+      intros.
+      eapply in_tchildren__in_schildren in Hin; eauto.
+      destruct Hin as [sdt [Hin Hconv]].
+      eapply forall_parent_children__in_children in Hin; eauto.
+      apply sdtree_tdtree__s2t_get_dtree_root in Hconv; eauto.
+  Case "nil".
+    inv Hconv. constructor.
+  Case "cons".
+    inv_mbind.
+    inv Hwf.
+    constructor; auto.
+Qed.
+
+Lemma wf_sdtree__wf_tdtree : forall (sdt:DTree) 
+  (Hwf: PDProps.wf_dtree ssuccs sentry Sdec sdt) tdt 
+  (Hconv: sdtree_tdtree sdt = Some tdt),
+  ADProps.wf_dtree tsuccs tentry Tdec tdt.
+Proof.
+  intros.
+  destruct wf_sdtree__wf_tdtree_mutrec as [J1 J2].
+  eapply J1; eauto.
+Qed.
+
+Hypothesis reachable_t2s: forall t (Hrd : ACfg.reachable tsuccs tentry t),
+  exists s, PTree.get s s2t = Some t /\ PCfg.reachable ssuccs sentry s.
+
+Hypothesis idom_t2s: forall t1 t2 
+  (Hrd : ACfg.reachable tsuccs tentry t2)
+  (Hidom: ADProps.idom tsuccs tentry t1 t2),
+  exists s1, exists s2,
+    PTree.get s1 s2t = Some t1 /\ PTree.get s2 s2t = Some t2 /\ 
+    PDProps.idom ssuccs sentry s1 s2.
+
+Lemma dtree_edge_iff_idom: forall (sdt:DTree) tdt
+  (Hconv: sdtree_tdtree sdt = Some tdt)
+  (Hcorrect: 
+    forall p0 ch0,
+    is_dtree_edge Sdec sdt p0 ch0 = true <-> 
+    (PCfg.imm_domination ssuccs sentry p0 ch0 /\ 
+     PCfg.reachable ssuccs sentry ch0)),
+  forall p0 ch0,
+    is_dtree_edge Tdec tdt p0 ch0 = true <-> 
+    (ACfg.imm_domination tsuccs tentry p0 ch0 /\ 
+    ACfg.reachable tsuccs tentry ch0).
+Proof.
+  intros.
+  split; intro J.
+    eapply is_tdtree_edge__ex_is_sdtree_edge in J; eauto.
+    destruct J as [sp [sch [J1 [J2 J3]]]].
+    apply Hcorrect in J3.
+    destruct J3 as [J3 J4].
+    split.
+      eapply idom_s2t; eauto.
+      eapply reachable_s2t; eauto.
+
+    destruct J as [J1 J2].
+    apply idom_t2s in J1; auto.
+    destruct J1 as [s1 [s2 [G1 [G2 G3]]]].
+    apply reachable_t2s in J2. destruct J2 as [s2' [G4 G5]].
+    assert (s2 = s2') as EQ.
+      eapply s2t_injective; eauto.
+    subst.
+    eapply is_sdtree_edge__is_tdtree_edge; eauto 1.
+    eapply Hcorrect; eauto.
+Qed.
+
+End DTreeConv.
+
+End DTreeConv.
+
+
